---
math: true
---

## Addition


$$
\begin{aligned}
&\forall x \;f(x, 0 ) =x \newline 
&\forall x \forall y \;f(x, S(y)) = S(f(x, y))
\end{aligned}
$$


## Multiplication

$$
\begin{aligned}
&h(x,0)\;:=\;0\newline 
&h\bigl(x,S(y)\bigr) \;:=\;f\bigl(h(x,y),\,x\bigr)
\end{aligned}
$$

Generated by AI.

## Statements

1. **Zero is neutral for addition**

   $$
   \forall x\;\bigl(x + 0 = x\bigr).
   $$

   *Every number plus zero is itself.*

2. **Successor distributes over addition**

   $$
   \forall x\,\forall y\;\bigl(x + S(y) = S(x + y)\bigr).
   $$

   *Adding the successor of $y$ to $x$ is the successor of $(x+y)$.*

3. **Zero annihilates multiplication**

   $$
   \forall x\;\bigl(x \cdot 0 = 0\bigr).
   $$

   *Any number times zero is zero.*

4. **Successor distributes over multiplication**

   $$
   \forall x\,\forall y\;\bigl(x \cdot S(y) = x\cdot y + x\bigr).
   $$

   *Multiplying by the successor is like multiplying and then adding once more.*

5. **Addition is commutative**

   $$
   \forall x\,\forall y\;\bigl(x + y = y + x\bigr).
   $$

   *Order doesn’t matter in addition.*

6. **Addition is associative**

   $$
   \forall x\,\forall y\,\forall z\;\bigl((x + y) + z = x + (y + z)\bigr).
   $$

   *You can reassociate sums freely.*

7. **Multiplication is commutative**

   $$
   \forall x\,\forall y\;\bigl(x \cdot y = y \cdot x\bigr).
   $$

   *Order doesn’t matter in multiplication either.*

8. **Distributive law**

   $$
   \forall x\,\forall y\,\forall z\;\bigl(x \cdot (y + z) = x\cdot y + x\cdot z\bigr).
   $$

   *Multiplication distributes over addition.*

9. **Cancellation law for addition**

   $$
   \forall x\,\forall y\,\forall z\;\bigl(x + z = y + z \;\rightarrow\; x = y\bigr).
   $$

   *If adding the same $z$ to two numbers yields equal sums, the numbers were equal.*

10. **Strictness of successor**

    $$
    \forall x\;\bigl(S(x) \neq 0\bigr).
    $$

    *No successor ever equals zero.*

11. **Injectivity of successor**

    $$
    \forall x\,\forall y\;\bigl(S(x) = S(y) \;\leftrightarrow\; x = y\bigr).
    $$

    *Different numbers have different successors.*

12. **The Induction Schema**
    For any formula $\varphi(x)$ in the language of PA one has the axiom‐schema instance

    $$
    \bigl[\;\varphi(0)\;\wedge\;\forall x\,( \varphi(x)\rightarrow \varphi(S(x)))\bigr]\;\rightarrow\;\forall x\,\varphi(x).
    $$

    *If a property holds of 0 and is preserved by successor, then it holds of all naturals.*

## Proofs

Below are sketch‐proofs—using only the Peano axioms plus the usual defining equations for “+” and “·” and the induction schema—of

1. Associativity of addition
2. Commutativity of addition
3. Associativity of multiplication
4. Commutativity of multiplication

For reference, the defining axioms are:

$$
\begin{aligned}
&x+0 = x,\\
&x + S(y) = S(x+y),\\
&x\cdot 0 = 0,\\
&x\cdot S(y) = x\cdot y + x,
\end{aligned}
$$

and induction is:

$$
\bigl[\varphi(0)\wedge\forall n\,(\varphi(n)\to\varphi(S(n)))\bigr]\;\to\;\forall n\,\varphi(n).
$$

---

## 1. Associativity of addition

**Theorem.**

$$
\forall x\,\forall y\,\forall z\;\bigl(x + (y + z) = (x + y) + z\bigr).
$$

**Proof (by induction on $z$).**

* **Base** $z=0$:

  $$
  x + (y+0) = x + y
  \quad\text{and}\quad
  (x+y)+0 = x+y
  $$

  by the defining clause $y+0=y$ and then $w+0=w$.

* **Inductive step**: assume

  $$
  x + (y + z) = (x + y) + z
  \quad\text{for some }z,
  $$

  and prove for $S(z)$:

  $$
  \begin{aligned}
    x + \bigl(y + S(z)\bigr)
    &= x + S\bigl(y+z\bigr)\quad(\text{by def.})\\
    &= S\bigl(x + (y+z)\bigr)\quad(\text{by def.})\\
    &= S\bigl((x+y) + z\bigr)\quad(\text{IH})\\
    &= (x+y) + S(z)\quad(\text{by def.}),
  \end{aligned}
  $$

  completing the induction.  ∎

---

## 2. Commutativity of addition

**Theorem.**

$$
\forall x\,\forall y\;\bigl(x + y = y + x\bigr).
$$

We first prove two helper lemmas.

**Lemma 2.1.** $\forall x\;(0 + x = x).$

* **By induction on $x$.**

  * Base $x=0$: $0+0=0$.
  * Step: $0+S(k)=S(0+k)=S(k)$ by def. and IH.

**Lemma 2.2.** $\forall x\,\forall y\;(S(x) + y = S(x+y)).$

* **By induction on $y$.**

  * Base $y=0$: $S(x)+0 = S(x)$ and $S(x+0)=S(x)$.
  * Step:

    $$
    \begin{aligned}
      S(x) + S(k)
      &= S\bigl(S(x)+k\bigr)\quad(\text{def.})\\
      &= S\bigl(S(x+k)\bigr)\quad(\text{IH})\\
      &= S\bigl(x + S(k)\bigr)\quad(\text{def.}),
    \end{aligned}
    $$

    so both sides agree.

Now the main proof by induction on $y$:

* **Base** $y=0$:

  $$
  x + 0 = x
  \quad\text{and}\quad
  0 + x = x
  $$

  by the defining equations and Lemma 2.1.

* **Step** assume $x + k = k + x$.  Then

  $$
  \begin{aligned}
    x + S(k)
    &= S\bigl(x + k\bigr)\quad(\text{def.})\\
    &= S\bigl(k + x\bigr)\quad(\text{IH})\\
    &= S(k) + x\quad(\text{Lemma 2.2 with }x\mapsto k,\;y\mapsto x).
  \end{aligned}
  $$

  Hence $x + S(k) = S(k) + x$.  ∎

---

## 3. Associativity of multiplication

**Theorem.**

$$
\forall x\,\forall y\,\forall z\;\bigl(x\cdot(y\cdot z) = (x\cdot y)\cdot z\bigr).
$$

**Proof (by induction on $z$).**

* **Base** $z=0$:

  $$
  x\cdot (y\cdot 0) = x\cdot 0 = 0
  \quad\text{and}\quad
  (x\cdot y)\cdot 0 = 0.
  $$
* **Step** assume $x\cdot(y\cdot k) = (x\cdot y)\cdot k$.  Then

  $$
  \begin{aligned}
    x\cdot\bigl(y\cdot S(k)\bigr)
    &= x\cdot\bigl(y\cdot k + y\bigr)\quad(\text{def. on mult.})\\
    &= x\cdot(y\cdot k) + x\cdot y\quad(\text{distributivity})\\
    &= (x\cdot y)\cdot k + x\cdot y\quad(\text{IH})\\
    &= (x\cdot y)\cdot S(k)\quad(\text{def. on mult.}),
  \end{aligned}
  $$

  completing the induction.  ∎

---

## 4. Commutativity of multiplication

**Theorem.**

$$
\forall x\,\forall y\;\bigl(x\cdot y = y\cdot x\bigr).
$$

We first note the lemma $\forall x\,(0\cdot x = 0)$, which is proved by induction on $x$ exactly like Lemma 2.1 above.

Then induct on $y$:

* **Base** $y=0$:

  $$
  x\cdot 0 = 0
  \quad\text{and}\quad
  0\cdot x = 0.
  $$

* **Step** assume $x\cdot k = k\cdot x$.  Then

  $$
  \begin{aligned}
    x\cdot S(k)
    &= x\cdot k + x\quad(\text{def.})\\
    &= k\cdot x + x\quad(\text{IH})\\
    &= x + k\cdot x\quad(\text{commutativity of + from §2})\\
    &= S(k)\cdot x\quad(\text{def. on mult.}).
  \end{aligned}
  $$

  Hence $x\cdot S(k) = S(k)\cdot x$.  ∎


## Predicates

1. **Zero**

   $$
   \mathrm{Zero}(x)\;\equiv\;x=0.
   $$

2. **Successor**

   $$
   \mathrm{Succ}(x,y)\;\equiv\;y=S(x).
   $$

3. **One**

   $$
   \mathrm{One}(x)\;\equiv\;x=S(0)\;=\;\overline{1}.
   $$

4. **Addition**

   $$
   \mathrm{Add}(x,y,z)\;\equiv\;x + y = z.
   $$

5. **Multiplication**

   $$
   \mathrm{Mul}(x,y,z)\;\equiv\;x \times y = z.
   $$

6. **Less-than**

   $$
   x < y \;\equiv\;\exists z\bigl(z \neq0\;\wedge\; x + z = y\bigr).
   $$

7. **Less-or-equal**

   $$
   x \le y \;\equiv\;\exists z\,(x + z = y).
   $$

8. **Divisibility**

   $$
   x\mid y \;\equiv\;\exists z\,(x \times z = y).
   $$

9. **Evenness**

   $$
   \mathrm{Even}(x)\;\equiv\;\exists y\,(x = y + y).
   $$

10. **Oddness**

    $$
    \mathrm{Odd}(x)\;\equiv\;\exists y\bigl(x = (y + y) + S(0)\bigr).
    $$

11. **Square-number**

    $$
    \mathrm{Square}(x)\;\equiv\;\exists y\,(y \times y = x).
    $$

12. **Prime**

    $$
    \mathrm{Prime}(x)\;\equiv\;x \neq0\;\wedge\;x \neq S(0)\;\wedge\;\forall y\forall z\Bigl(x = y\times z \;\rightarrow\;(y = S(0)\;\lor\;z = S(0))\Bigr).
    $$

13. **Factorial**

    $$
    \mathrm{Fact}(n,m)\;\equiv\;\bigl[n=0\wedge m=S(0)\bigr]\;\lor\;\exists u\exists v\bigl[n=S(u)\wedge \mathrm{Fact}(u,v)\wedge m = S(u)\times v\bigr].
    $$

14. **Power of 2**

    $$
    \mathrm{Pow2}(x)\;\equiv\;\bigl[x = S(0)\bigr]\;\lor\;\exists y\bigl(\mathrm{Pow2}(y)\;\wedge\;x = y + y\bigr).
    $$

15. **Exponentiation** (as a ternary relation)

    $$
    \mathrm{Exp}(a,b,c)\;\equiv\;\bigl[b=0\wedge c=S(0)\bigr]\;\lor\;\exists u\exists v\bigl[b=S(u)\wedge \mathrm{Exp}(a,u,v)\wedge c = a \times v\bigr].
    $$

## Proofs

---

### 1. $ \displaystyle PA\;\vdash\;\forall x\,(x + 0 = x)$

We prove by induction on $x$.

$$
\begin{aligned}
\text{(Axiom)}\quad& x + 0 = x &&\text{is one of the defining axioms of \(+\).}\newline
\text{Base case:}&\quad 0 + 0 = 0 &&\text{instantiate the axiom at \(x:=0\).}\newline
\text{Inductive step:}&\quad\text{Assume }u + 0 = u.\newline
&\quad S(u) + 0 = S\bigl(u + 0\bigr) &&\text{by the axiom }x + 0 = x\text{ with }x:=S(u).\newline
&\quad\;\;=\;S(u) &&\text{by the inductive hypothesis.}\newline
&\quad\text{Hence }(S(u)+0 = S(u)).\newline
\text{By Induction:}&\quad PA\vdash\forall x\,(x+0=x).
\end{aligned}
$$

---

### 2. $ \displaystyle PA\;\vdash\;\forall x\,(x \le x)$

Recall $x\le y$ is defined as $\exists z\,(x+z = y)$.

$$
\begin{aligned}
&\text{Fix an arbitrary \(x\).}\newline
&\text{We exhibit the witness \(z:=0\).}\newline
&\quad x + 0 = x &&\text{by the axiom just proved above.}\newline
&\therefore\;\exists z\,(x+z = x).\newline
&\text{Since \(x\) was arbitrary, }PA\vdash\forall x\,(x\le x).
\end{aligned}
$$

No induction needed beyond our previous theorem.

---

### 3. $ \displaystyle PA\;\vdash\;\forall x\,\forall y\,\forall z\;\bigl(x<y \wedge y<z \;\to\; x<z\bigr)$

Here $x<y$ is shorthand for
$\exists u\,[u\neq0\wedge x+u = y]$.

$$
\begin{aligned}
&\text{Fix \(x,y,z\), and assume }x<y\wedge y<z.\newline
&\text{Then }\exists u\bigl(u\neq0\wedge x+u=y\bigr),\quad\exists v\bigl(v\neq0\wedge y+v=z\bigr).\newline
&\text{Unpack both existentials: let \(u,v\) satisfy those.}\newline
&\text{Define }w := u+v.\newline
&\quad w\neq0 \newline
&\quad x+w 
   = x + (u+v)
   = (x+u) + v
   = y + v
   = z \newline
&\text{Hence }\exists w\,\bigl(w\neq0\wedge x+w=z\bigr),\text{ i.e.\ }x<z.\newline
&\text{By generalizing over \(x,y,z\),}
  \;PA\vdash\forall x\,\forall y\,\forall z\,(x<y\wedge y<z\to x<z).
\end{aligned}
$$

